experiment/Experiment.Steel.fst
@@ -14,13 +14,12 @@ module SF2Fun = Experiment.Steel.Repr.SF_to_Fun
 
 #push-options "--ifuel 0 --fuel 0"
 let prog_LV_to_Fun_equiv_M
-      (#ek : SH.effect_kind) (#a : Type) (t : M.repr ek a)
+      (#a : Type) (t : M.prog_tree a)
       (#pre : M.pre_t) (#post : M.post_t a)
-      (lc : LV.top_lin_cond t.repr_tree pre post {LV.lcsub_at_leaves lc})
+      (lc : LV.top_lin_cond t pre post {LV.lcsub_at_leaves lc})
       (sl0 : Vpl.sl_f pre)
-  : Lemma (prog_M_equiv_Fun t.repr_tree (LV2M.repr_M_of_LV_top lc) sl0 (prog_LV_to_Fun t lc sl0))
+  : Lemma (prog_M_equiv_Fun t (LV2M.repr_M_of_LV_top lc) sl0 (prog_LV_to_Fun t lc sl0))
   =
-    let tr    = t.repr_tree                  in
     let mc    = LV2M.repr_M_of_LV_top lc     in
     let sl0_l = Fl.dlist_of_f sl0            in
     let t_SF  = LV2SF.repr_SF_of_LV lc sl0_l in
@@ -30,14 +29,19 @@ let prog_LV_to_Fun_equiv_M
     LV2SF.repr_SF_of_LV_sound lc sl0_l;
     SF2Fun.repr_Fun_of_SF_req t_SF;
 
-    let lem_req () : Lemma (M.tree_req t.repr_tree mc sl0 <==> Fun.tree_req t_Fun) = () in
+    let lem_req () : Lemma (M.tree_req t mc sl0 <==> Fun.tree_req t_Fun) = () in
     let lem_ens (x : a) (sl1 : Vpl.sl_f (post x))
-      : Lemma (M.tree_ens tr mc sl0 x sl1 <==> Fun.tree_ens t_Fun ({val_v = x; sel_v = sl1}))
+      : Lemma (M.tree_ens t mc sl0 x sl1 <==> Fun.tree_ens t_Fun ({val_v = x; sel_v = sl1}))
       = SF2Fun.repr_Fun_of_SF_ens t_SF x sl1
     in
-    assert (prog_M_equiv_Fun t.repr_tree (LV2M.repr_M_of_LV_top lc) sl0 (prog_LV_to_Fun t lc sl0))
+    assert (prog_M_equiv_Fun t (LV2M.repr_M_of_LV_top lc) sl0 (prog_LV_to_Fun t lc sl0))
       by (norm [delta_only [`%prog_M_equiv_Fun]];
           split ();
             apply_lemma (``@lem_req);
             let _ = mintros () in apply_lemma (``@lem_ens))
 #pop-options
+
+(**) #push-options "--no_tactics"
+(**) private let __begin_build_to_steel_wrew = ()
+(**) #pop-options
+(**) private let __end_build_to_steel_wrew = ()
